Cleaning up

proof/correctness/R256.ec
@@ -11,27 +11,13 @@ lemma to_sintD_small : (forall (a b : W16.t),
 proof. 
 move => a b.
   rewrite !W16.to_sintE !/smod => />.
-  move : (W16.to_uint_cmp a). 
-  move : (W16.to_uint_cmp b). 
-  case(32768 <= to_uint a).
-  case(32768 <= to_uint b).
-  move => /> *.  
-  rewrite (_:  to_uint (a + b)= (to_uint a +  to_uint b) - 65536).
-  rewrite to_uintD => />;   smt(@W16).  smt(@W16).
-  move => /> *. 
+  move : (W16.to_uint_cmp a) (W16.to_uint_cmp b) => *.
+  have sumbnd : to_uint a + to_uint b < 65536+65536; first  by smt. 
   case (65536  <= to_uint a + to_uint b).
-  move => *.
-  rewrite (_:  to_uint (a + b)= (to_uint a +  to_uint b) - 65536).
-  rewrite to_uintD => />;   smt(@W16).  smt(@W16).
-  move => *.  
-  rewrite to_uintD_small => />;   smt(@W16).  
-  move => /> *. 
-  case (65536  <= to_uint a + to_uint b).
-  move => *.
-  rewrite (_:  to_uint (a + b)= (to_uint a +  to_uint b) - 65536).
-  rewrite to_uintD => />;   smt(@W16).  smt(@W16).
-  move => *.  
-  rewrite to_uintD_small => />;   smt(@W16).  
++    move => *; rewrite (_:  to_uint (a + b)= (to_uint a +  to_uint b) - 65536);
+       [rewrite to_uintD => />; by  smt(@IntDiv @W16) |  smt(@W16)].
++    move => *; rewrite (_:  to_uint (a + b)= (to_uint a +  to_uint b));
+       [rewrite to_uintD_small => />; by  smt(@IntDiv @W16) |  smt(@W16)].
 qed.
 
 
@@ -39,27 +25,16 @@ lemma to_sintB_small : (forall (a b : W16.t),
     -W16.modulus %/2 <= to_sint a - to_sint b < W16.modulus %/2 =>
     to_sint (a - b) = to_sint a - to_sint b).
 proof.
-move => a b.
+  move => a b.
   rewrite !W16.to_sintE !/smod => />.
-  move : (W16.to_uint_cmp a). 
-  move : (W16.to_uint_cmp b). 
+  move : (W16.to_uint_cmp a) (W16.to_uint_cmp b). 
   case (to_uint b <= to_uint a).
-  move => /> *.  
-  case(32768 <= to_uint a).
-  rewrite (_:  to_uint (a - b)= (to_uint a -  to_uint b)); smt(@W16 @IntDiv).
-  rewrite (_:  to_uint (a - b)= (to_uint a -  to_uint b)); smt(@W16 @IntDiv).
-  move => /> *.  
-  case(32768 <= to_uint a).
-  case(32768 <= to_uint b).
-  move => /> *.  
-  rewrite (_:  to_uint (a - b)= (to_uint a -  to_uint b) + 65536).
-  rewrite to_uintD to_uintN => />;  smt(@W16 @IntDiv). smt(@W16 @IntDiv).
-  move => /> *.  
-  rewrite (_:  to_uint (a - b)= (to_uint a -  to_uint b) + 65536).
-  rewrite to_uintD to_uintN => />;  smt(@W16 @IntDiv). smt(@W16 @IntDiv).
-  move => /> *.  
-  rewrite (_:  to_uint (a - b)= (to_uint a -  to_uint b) + 65536).
-  rewrite to_uintD to_uintN => />;  smt(@W16 @IntDiv). smt(@W16 @IntDiv).
++ case(32768 <= to_uint a); 
+    by move => *;
+      rewrite (_:  to_uint (a - b)= (to_uint a -  to_uint b)); smt(@W16 @IntDiv).
++ case(32768 <= to_uint a);  by 
+    move => /> *; rewrite (_:  to_uint (a - b)= (to_uint a -  to_uint b) + 65536);
+      [rewrite to_uintD to_uintN => />;  smt(@W16 @IntDiv)| smt(@W16 @IntDiv)].
 qed.
 
 lemma to_sintM_small : (forall (a b : W16.t), 
@@ -68,22 +43,11 @@ lemma to_sintM_small : (forall (a b : W16.t),
 proof.
 move => a b.
   rewrite !W16.to_sintE !/smod => />.
-  move : (W16.to_uint_cmp a). 
-  move : (W16.to_uint_cmp b). 
-  case(32768 <= to_uint a).
-  case(32768 <= to_uint b).
-  move => /> *; smt(@W16).
-  move => *.
-  case (65536  <= to_uint a * to_uint b).
-  rewrite to_uintM  => />;  smt(@W16 @IntDiv). 
-  smt(@W16 @IntDiv).
-  move => *.
-  case(32768 <= to_uint b).
-  case (65536  <= to_uint a * to_uint b).
-  move => *.
-  rewrite to_uintM  => />;  smt(@W16 @IntDiv). 
-  smt(@W16 @IntDiv).
-  rewrite to_uintM  => />;  smt(@W16 @IntDiv). 
+  move : (W16.to_uint_cmp a) (W16.to_uint_cmp b) => *.
+  case(32768 <= to_uint a);
+    case(32768 <= to_uint b);
+      by case (65536  <= to_uint a * to_uint b);
+       move => *;rewrite to_uintM  => />;  smt(@W16 @IntDiv). 
 qed.
 
 (*
@@ -119,15 +83,23 @@ import Fq.
 import ZModP.
 
 op q = W16.of_int 3329 axiomatized by qE.
+op b16 (a : W16.t) (b : int) = 
+     -b <= to_sint a < b axiomatized by b16E.
+
+op bpos16 (a : W16.t) (b : int) = 
+     0 <= to_sint a < b  axiomatized by bpos16E.
 
 op bw16 (a : W16.t) i =
-     0 <= i <= 15 /\ (* signed 15 bits at most *)
-     -2^i <= to_sint a < 2^i.
+     -2^i <= to_sint a < 2^i  axiomatized by bw16E.
+
+hint simplify b16E.
+hint simplify bpos16E.
+hint simplify bw16E.
 
 op add (a b : W16.t) = (a + b).
 
 lemma add_corr (a b : W16.t) (a' b' : zmod) (asz bsz : int): 
-   asz < 15 => bsz < 15 =>
+   0 <= asz < 15 => 0 <= bsz < 15 =>
    a' = inzmod (W16.to_sint a) =>
    b' = inzmod (W16.to_sint b) =>
    bw16 a asz => 
@@ -135,28 +107,23 @@ lemma add_corr (a b : W16.t) (a' b' : zmod) (asz bsz : int):
      inzmod (W16.to_sint (add a b)) = a' + b' /\
            bw16 (add a b) (max asz bsz + 1).
 proof.
-
-rewrite /bw16 /add  => />.
+rewrite /add  => />.
 pose aszb := 2^asz.
 pose bszb := 2^bsz.
-move => ?? ?? [#?] ?? [#?] ??.
-
-have bounds_asz : 0 < aszb <= 16384; first by split; [ apply gt0_pow2 | move => *; apply (pow_Mle asz 14 _) => /# ].
-have bounds_bsz : 0 < bszb <= 16384; first by split; [ apply gt0_pow2 | move => *; apply (pow_Mle bsz 14 _) => /#].
-
-rewrite !to_sintD_small; first by smt().
+move => ?? ?? ?? ??.
+have bounds_asz : 0 < aszb <= 16384;
+  first by split; [ apply gt0_pow2 | move => *; apply (pow_Mle asz 14 _) => /#].
+have bounds_bsz : 0 < bszb <= 16384; 
+  first by split; [ apply gt0_pow2 | move => *; apply (pow_Mle bsz 14 _) => /#].
+rewrite !to_sintD_small => />; first by  by smt().
 
 split; first by smt(@ZModP).
-split; first by smt().
 
-case ( max asz bsz = asz).
-move => *; rewrite H9. 
-rewrite (_: 2^(asz + 1) = aszb * 2). smt(@IntExtra). 
-have ? : (- aszb  <= to_sint b); smt(@W16 @IntExtra).
-
-move => *. rewrite (_: max asz bsz = bsz). smt(). 
-rewrite (_: 2^(bsz + 1) = bszb * 2). smt(@IntExtra). 
-have ? : (- bszb  <= to_sint a); smt(@W16 @IntExtra).
+case (max asz bsz = asz).
++ move => maxx; rewrite maxx;
+  rewrite (_: 2^(asz + 1) = aszb * 2); smt(@W16 @IntExtra). 
++ move => maxx; rewrite (_: max asz bsz = bsz); 
+    [by smt() | by rewrite (_: 2^(bsz + 1) = bszb * 2); smt(@W16 @IntExtra)]. 
 qed.
 
 import Fq.SignedReductions.
@@ -196,14 +163,9 @@ while (0 <= to_uint j <= 256 /\
 auto => />. 
 move => &ht H.
 split; first by smt().
-move => *. 
-move : H; rewrite ultE of_uintK => />; smt(@W16 @W64).
-move => *.
-wp. sp.
-exists* t, j.
-elim* => t j.
-call (barret_reduct_corr _a.[to_uint j]).
-by auto => />;smt(@W64 @Array256).
+move => ??; move : H; rewrite ultE of_uintK => />; smt(@W16 @W64).
+move => *;wp; sp; exists* t, j; elim* => t j; call (barret_reduct_corr _a.[to_uint j]); 
+ auto => />;smt(@W64 @Array256).
 qed.
 
 op lift_array (p : W16.t Array256.t) =
@@ -219,17 +181,13 @@ axiom load_array_from_memE mem ptr i :
      loadW16 mem (W64.to_uint ptr + 2* i) = (load_array_from_mem mem ptr).[i].
 
 op ntt_bound_zetas(zetas : W16.t Array256.t) : bool =
-   forall k, 0 <= k < 256 => 0 <= to_sint zetas.[k] < Fq.q-1.
+   forall k, 0 <= k < 256 => bpos16  zetas.[k] (Fq.q-1).
 
 op log2(n : int) : int.
 
 (* TODO: use easycrypt's native log to base *)
-axiom log2E n l :
-   0 <= l => n = 2^l => log2 n = l.
-
-axiom log2pos n :
-   1 <= n => 0 <= log2 n.
-
+axiom log2E n l : 0 <= l => n = 2^l => log2 n = l.
+axiom log2pos n : 1 <= n => 0 <= log2 n.
 
 lemma logs :
    log2 128 = 7 /\
@@ -245,13 +203,10 @@ lemma logs :
 lemma logdiv2 n l :
   1 < n =>
   n = 2^l =>
-  log2 (n %/2) = log2 n -1
-   by smt(@IntExtra log2E). 
-
+  log2 (n %/2) = log2 n - 1 by smt(@IntExtra log2E). 
 
 op ntt_bound_coefs(coefs : W16.t Array256.t, l u c : int) : bool =
-   forall k, l <= k < u => -c*Fq.q <= to_sint coefs.[k] <= c*Fq.q.
-
+   forall k, l <= k < u => b16 coefs.[k] (c*Fq.q).
 
 equiv ntt_correct &m :
   NTT_Fq.NTT.ntt ~ M.poly_ntt : 
@@ -263,12 +218,11 @@ equiv ntt_correct &m :
         ntt_bound_coefs rp{2} 0 256 2
           ==> 
             res{1} = lift_array res{2} /\
-            all (fun x => 0<= W16.to_sint x < 2*Fq.q) res{2}.
+            all (fun x => bpos16 x (2*Fq.q)) res{2}.
 proc.
 (* Dealing with final barret reduction *)
 seq 3 2 :  (forall k, 0 <= k < 256 => r{1} = lift_array rp{2}); last first.
-exists * r{1}, rp{2}.
-elim* => r1 rp2.
+exists * r{1}, rp{2}; elim* => r1 rp2.
 call {2} (_:  
      forall i, 0 <= i < 256 =>
              to_sint rp.[i] = (map (fun (x : W16.t) => to_sint x) rp2).[i]
@@ -277,33 +231,30 @@ call {2} (_:
              to_sint res.[i] =
              BREDC (map (fun (x : W16.t) => to_sint x) rp2).[i] 26). 
 apply (poly_reduct_corr (Array256.map (fun x => (W16.to_sint x)) rp2)).
-skip. move => &1 &2 [#] ???.
-split.
-move => i ibnd; first by smt (@Array256).
+skip; move => &1 &2 [#] ???.
+split; first by smt (@Array256).
+
 move => ???.
-have bnds : (
- forall (k : int),
-      0 <= k < 256 =>
-      -32768 <= to_sint rp{2}.[k] < 32768
-). 
-move => k kb. rewrite to_sintE /smod => />. 
-move : (W16.to_uint_cmp ( rp{2}.[k]));smt().
+have bnds : (forall k, 0 <= k < 256 => bw16 rp{2}.[k] 15). 
+by move => k kb />; rewrite to_sintE /smod => />;
+      move : (W16.to_uint_cmp ( rp{2}.[k]));smt().
+
 split.
 
 + rewrite (Array256.ext_eq r{1} (lift_array result)) //=.
    move => x xb;rewrite /lift_array  mapiE //=  (H3 x xb) mapiE => />.
    move : (BREDCp_corr (to_sint rp2.[x]) 26 _ _ _ _ _);
-      first 5 by smt(@Fq).  
+      first 5 by smt(@Fq bw16E).  
    move : (H1 x xb);rewrite Array256.tP => [# ] ? [#] ???.
    move : (H4 x xb);rewrite /lift_array mapiE => /> *;smt(@ZModP).
-+ rewrite allP => i ib />.  
-  rewrite  (H3 i ib) mapiE => />.
-  move : (BREDCp_corr (to_sint rp2.[i]) 26 _ _ _ _ _);smt(@Fq @ZModP).
+
++ rewrite allP => i ib />; rewrite (H3 i ib) mapiE => />.
+  move : (BREDCp_corr (to_sint rp2.[i]) 26 _ _ _ _ _);smt(@Fq @ZModP bw16E).
 (***********************************)
 
-sp.
-exists *zetasp{2}.
-elim* => zetasp2.
+sp;exists *zetasp{2};elim* => zetasp2.
+
+(* Outer loop *)
 while (
    to_uint zetasp{2} + 512 - (k{1}-1)*2 < W64.modulus /\
    r{1} = lift_array rp{2} /\
@@ -315,11 +266,12 @@ while (
    to_uint zetasp{2} = to_uint zetasp2 + (k{1}-1)*2 /\
    2*k{1}*len{1} = 256 /\
    ntt_bound_zetas (load_array_from_mem Glob.mem{2} zetasp2) /\ 
-   ntt_bound_coefs rp{2} 0 256 (9 - log2 len{1})); last by  auto => />; smt.
-wp.
-exists* k{1}.
-elim* => k1.
-move  => l.
+   ntt_bound_coefs rp{2} 0 256 (9 - log2 len{1})); last by
+    auto => />; move => *; split; [ by smt() |
+                           split; [exists 7 => />; smt()| by smt(logs log2E)]].
+wp; exists* k{1}; elim* => k1 l.
+
+(* Middle loop *)
 while (#{/~k1=k{1}}
         {~2*k{1}*len{1} = 256}
         {~ntt_bound_coefs rp{2} 0 256 (9 - log2 len{1})}pre /\ 
@@ -332,19 +284,17 @@ while (#{/~k1=k{1}}
        ntt_bound_coefs  rp{2} 0 256 (9 - log2 len{1} + 1) /\
        ntt_bound_coefs  rp{2} start{1} 256 (9 - log2 len{1})
        ); last first.
- auto => />; move => *.
-split; first by smt(@W16 @Array256 @Fq).
-move => *.
-rewrite uleE !shr_div.
-split; last  by smt(@W64).
-split; first  by smt(@W64).
-split; first by  exists (l-1); smt(@IntExtra).
-split; first  by smt(@W64). 
-rewrite (logdiv2 (to_uint len{2}) (log2 (to_uint len{2}))). smt(@W16). 
- smt. (* mistery *)
-by smt(@W16 @Array256 @Fq).
+auto => />; move => *.
+split; first by move : H9; rewrite /ntt_bound_coefs => />; smt(@Fq).
+move => *;rewrite uleE !shr_div => />.
+split; last by  
+   rewrite (logdiv2 (to_uint len{2}) (log2 (to_uint len{2}))); 
+    [ smt(@W64) | smt(log2E) | smt(@W64) ]. 
+ by  exists (l-1); smt(@IntExtra).
 
 wp.
+
+(* Inner loop *)
 while (#{/~start{1} = 2*(k{1} - k1) * len{1}}
         {~ntt_bound_coefs  rp{2} start{1} 256 (9 - log2 len{1})} pre /\
        zeta_{1}  *  (inzmod R) = inzmod (to_sint zeta_0{2}) /\  
@@ -357,350 +307,136 @@ while (#{/~start{1} = 2*(k{1} - k1) * len{1}}
        ntt_bound_coefs  rp{2} (j{1}) (start{1} + len{1}) (9 - log2 len{1}) /\
        ntt_bound_coefs  rp{2} (j{1} + len{1}) 256 (9 - log2 len{1})
        )
-       );last first. auto => />. 
-move => &1 &2 ????????????????????.
+       );last first. 
+auto => />. 
+move => &1 &2 ?? ?? lenpow2 ?? ?? ??????? cbdloose cbdtight ?? => />.
+
 split.
+
+(* Initialization *) 
 split; last by rewrite ultE to_uintD_small; by smt(@W64).
+split; first by  rewrite !to_uintD_small of_uintK => />;smt(@IntExtra @W64).
+
 split. 
-split; first by rewrite !to_uintD_small of_uintK => />;smt(@IntExtra @W64).
-split; first by smt(@W64).
-split; last by rewrite to_uintD_small; by smt(@W64). 
-by smt(@W64).
-split. 
-rewrite to_uintD_small => />; first by smt(@W64). 
-rewrite H6 => />.
+rewrite to_uintD_small H5 => />; first by smt(@W64). 
 rewrite (_: 
    (to_uint zetasp2 + (k{1} - 1) * 2 + 2) = 
-   (to_uint zetasp2 + 2 * k{1} )). by ring. 
-rewrite (load_array_from_memE (Glob.mem{2}) ( zetasp2) (k{1})) => />.
-smt(@Array256 @ZModP).
-move : H0; rewrite /array_mont.
-by smt(@ZModP @Array256).
-split.
-move : H7; rewrite /ntt_bound_zetas => AA; move : (AA (k{1}) _). smt().
-rewrite -(load_array_from_memE (Glob.mem{2}) zetasp2). smt().
-rewrite (_: to_uint (zetasp{2} + (of_int 2)%W64) = to_uint zetasp2 + 2 * k{1}).
-rewrite to_uintD_small; smt(@W64). smt(@W64).
-split; first by rewrite to_uintD_small; by smt(@W64). 
-split; first by smt(@W64).
-split; last by smt(@W16 @Array256 @Fq).
-have ? : ((to_uint start{2} + to_uint len{2}) < 256);by smt(@W16 @Array256 @Fq).
+   (to_uint zetasp2 + 2 * k{1} )); first by ring. 
+rewrite (load_array_from_memE (Glob.mem{2}) ( zetasp2) (k{1})) //= /array_mont; smt(@Array256 @ZModP).
 
+split.
+move : H6; rewrite /ntt_bound_zetas => AA; move : (AA (k{1}) _); first by smt().
+rewrite -(load_array_from_memE (Glob.mem{2}) zetasp2); first by smt().
+rewrite (_: to_uint (zetasp{2} + (of_int 2)%W64) = to_uint zetasp2 + 2 * k{1}); [ by rewrite to_uintD_small; smt(@W64) | by smt(@W64)].
+by rewrite to_uintD_small; have ? : ((to_uint start{2} + to_uint len{2}) < 256);by smt(@W16 @Array256 @Fq).
+
+(* Termination *)
 move => *.
 split.
-split; first by rewrite !to_uintD_small => />;  by smt(@W64).
-split; last first. 
-rewrite (_:to_uint j_R = to_uint start{2} + to_uint len{2}).
-smt(). ring. rewrite H13. by ring.
-split; first   by smt(@W64).
-move => *. 
-rewrite (_:to_uint j_R = to_uint start{2} + to_uint len{2}).
-smt(@W64).  rewrite H13. 
-have stronger : (2*(k{1}+1)*to_uint len{2}  <= 512); smt().
-split.  move => * />. 
-rewrite ultE /of_uingK => />.
-rewrite to_uintD_small. smt(@W64). smt(@W64). 
-rewrite ultE /of_uingK => />.
-rewrite to_uintD_small. smt(@W64). 
-smt(@W64).
+rewrite (_:to_uint j_R = to_uint start{2} + to_uint len{2}); first by smt().
+split; [ by rewrite !to_uintD_small => />;  by smt(@W64) | by smt(@W64) ].
+by rewrite ultE /of_uingK to_uintD_small; smt(@W64).
 
-wp. sp.
-exists* t{2}, zeta_0{2}.
-elim* => t2 zeta_02.
+(* Preservation *)
+wp; sp; exists* t{2}, zeta_0{2}; elim* => t2 zeta_02.
 call {2} (_:
    to_sint a = to_sint t2 /\ to_sint b = to_sint zeta_02   
    ==> 
   to_sint res = SREDC (to_sint t2 * to_sint zeta_02)
-). apply (fqmul_corr (to_sint t2) (to_sint zeta_02)).
+); first by apply (fqmul_corr (to_sint t2) (to_sint zeta_02)).
 skip => />.
-move => &1 &2 [#] ?? ?? ?? ?? ?? ?? ???????????????????.
+move => &1 &2 [#] ?? ?? ?? ?? bzetas ???? ?? bloose ?? zetaval ?? -> cmp ?? btightsmall btightlarge ??? resval.
+
+move : btightlarge; rewrite /ntt_bound_coefs => /> btightlarge. 
+ move : (btightlarge (to_uint (j{2} + len{2})) _);
+ rewrite to_uintD_small; first 3 by smt(@W16).  
+move : btightsmall; rewrite /ntt_bound_coefs => /> btightsmall. 
+ move : (btightsmall (to_uint (j{2})) _); first by smt(@W16).
+move => jbound jlenboundl llenboundh.
+
+have bound1 : 2 <= to_uint len{2}; first by smt().
+have bound2 : (9 - log2 (to_uint len{2})) * Fq.q <= 8*Fq.q; first by smt(@Fq logs).
+have bound3 : -8*Fq.q <=  to_sint rp{2}.[to_uint j{2} + to_uint len{2}]<= 8*Fq.q; first by smt().
+have bound4 : -8*Fq.q <=  to_sint rp{2}.[to_uint j{2}]<= 8*Fq.q; first by smt().
+
+move :resval; rewrite to_uintD_small; first by smt(@W64). move => resval.
+
+move : (SREDCp_corr (to_sint rp{2}.[to_uint j{2} + to_uint len{2}] * to_sint zeta_0{2}) _ _); 
+  first 2 by have ? : (-R %/ 2 * Fq.q < -8*Fq.q*Fq.q ); smt(@Fq). 
+rewrite -!resval. move => sredc.
+
 split; last by smt(@W64).
 split; last first.
 split; first by smt(@W64).
 split; first by smt().
+
 (********* bounding carries *)
 (* tighter bound *)
-move : H25; rewrite /ntt_bound_coefs => AA. 
- move : (AA (to_uint (j{2} + len{2})) _);
- rewrite to_uintD_small; first 3 by smt(@W16).  
-move : H24; rewrite /ntt_bound_coefs => BB. 
- move : (BB (to_uint (j{2})) _); first by smt(@W16).
 move => *.
 
 split; last first.
 (* part 1*)
 move => *.
-
-move => *.
-have ? : (2 <= to_uint len{2}). smt.
-have ? : ((9 - log2 (to_uint len{2})) * Fq.q <= 8*Fq.q). smt.
-
-have ? : -8*Fq.q <=  to_sint rp{2}.[to_uint j{2} + to_uint len{2}]<= 8*Fq.q. smt().
-have ? : -8*Fq.q <=  to_sint rp{2}.[to_uint j{2}]<= 8*Fq.q. smt().
-
-move : (SREDCp_corr (to_sint rp{2}.[to_uint j{2} + to_uint len{2}] * to_sint zeta_0{2}) _ _); first  by smt(@Fq). 
-have ? : (-R %/ 2 * Fq.q < -8*Fq.q*Fq.q ); smt(@Fq).
-
-case (k0 <> to_uint j{2} /\ k0 <> to_uint j{2} + to_uint len{2}).
-move => *; rewrite !Array256.set_neqiE; smt(@W64). 
-case (k0 = to_uint j{2}). 
-move => *;rewrite !Array256.set_eqiE; first 2 by smt(@W64). 
-rewrite to_sintD_small => /> *.
-
-
-move => *.  rewrite H28.
- rewrite to_uintD_small; first by smt(@W16).  
-have ? : (( Fq.q) + ( 8*Fq.q) < R %/ 2 );   by smt(@Fq). 
-smt().
-
-move => ??.
-rewrite (_:k0 = to_uint j{2} + to_uint len{2}); first by smt().
-move => *; rewrite Array256.set_neqiE; first 2 by smt(@W64). 
-move => *; rewrite Array256.set_eqiE; first 2 by smt(@W64). 
- rewrite to_sintB_small.
-
-move => *.  rewrite H28.
- rewrite to_uintD_small; first by smt(@W16).  
-have ? : (( Fq.q) + ( 8*Fq.q) < R %/ 2 );   by smt(@Fq). 
-smt().
-
+case (k0 <> to_uint j{2} /\ k0 <> to_uint j{2} + to_uint len{2}); first by 
+  move => *; rewrite !Array256.set_neqiE; smt(@W64). 
+  case (k0 = to_uint j{2}). 
+  move => *;rewrite !Array256.set_eqiE;  smt(@W64).
+  move => *; rewrite (_:k0 = to_uint j{2} + to_uint len{2}); first by smt().
+  rewrite Array256.set_neqiE; first 2 by smt(@W64). 
+  rewrite Array256.set_eqiE; by smt(@W64). 
 (* part 2 *)
 move => *.
+case (k0 <> to_uint j{2} /\ k0 <> to_uint j{2} + to_uint len{2}); first by 
+  move => *; rewrite !Array256.set_neqiE; smt(@W64). 
+  case (k0 = to_uint j{2}). 
+  move => *;rewrite !Array256.set_eqiE;  smt(@W64).
+  move => *; rewrite (_:k0 = to_uint j{2} + to_uint len{2}); first by smt().
+  rewrite Array256.set_neqiE; first 2 by smt(@W64). 
+  rewrite Array256.set_eqiE; by smt(@W64). 
 
-move => *.
-have ? : (2 <= to_uint len{2}). smt.
-have ? : ((9 - log2 (to_uint len{2})) * Fq.q <= 8*Fq.q). smt.
-
-have ? : -8*Fq.q <=  to_sint rp{2}.[to_uint j{2} + to_uint len{2}]<= 8*Fq.q. smt().
-have ? : -8*Fq.q <=  to_sint rp{2}.[to_uint j{2}]<= 8*Fq.q. smt().
-
-move : (SREDCp_corr (to_sint rp{2}.[to_uint j{2} + to_uint len{2}] * to_sint zeta_0{2}) _ _); first  by smt(@Fq). 
-have ? : (-R %/ 2 * Fq.q < -8*Fq.q*Fq.q ); smt(@Fq).
-
-case (k0 <> to_uint j{2} /\ k0 <> to_uint j{2} + to_uint len{2}).
-move => *; rewrite !Array256.set_neqiE; smt(@W64). 
-case (k0 = to_uint j{2}). 
-move => *;rewrite !Array256.set_eqiE; first 2 by smt(@W64). 
-rewrite to_sintD_small => /> *.
-
-
-move => *.  rewrite H28.
- rewrite to_uintD_small; first by smt(@W16).  
-have ? : (( Fq.q) + ( 8*Fq.q) < R %/ 2 );   by smt(@Fq). 
-smt().
-
-move => ??.
-rewrite (_:k0 = to_uint j{2} + to_uint len{2}); first by smt().
-move => *; rewrite Array256.set_neqiE; first 2 by smt(@W64). 
-move => *; rewrite Array256.set_eqiE; first 2 by smt(@W64). 
- rewrite to_sintB_small.
-
-move => *.  rewrite H28.
- rewrite to_uintD_small; first by smt(@W16).  
-have ? : (( Fq.q) + ( 8*Fq.q) < R %/ 2 );   by smt(@Fq). 
-smt().
-
-(* Looser bound *)
 split; last first.
+(* looser bound *)
 
-move : H25; rewrite /ntt_bound_coefs => AA. 
- move : (AA (to_uint (j{2} + len{2})) _);
- rewrite to_uintD_small; first 3 by smt(@W16).  
-move : H24; rewrite /ntt_bound_coefs => BB. 
- move : (BB (to_uint (j{2})) _); first by smt(@W16).
-move => *.
-
-have ? : (2 <= to_uint len{2}). smt.
-have ? : ((9 - log2 (to_uint len{2})) * Fq.q <= 8*Fq.q). smt.
-
-have ? : -8*Fq.q <=  to_sint rp{2}.[to_uint j{2} + to_uint len{2}]<= 8*Fq.q. smt().
-have ? : -8*Fq.q <=  to_sint rp{2}.[to_uint j{2}]<= 8*Fq.q. smt().
-
-move : (SREDCp_corr (to_sint rp{2}.[to_uint j{2} + to_uint len{2}] * to_sint zeta_0{2}) _ _); first  by smt(@Fq). 
-have ? : (-R %/ 2 * Fq.q < -8*Fq.q*Fq.q ); smt(@Fq).
-
-case (k0 <> to_uint j{2} /\ k0 <> to_uint j{2} + to_uint len{2}).
-move => *; rewrite !Array256.set_neqiE; smt(@W64). 
-case (k0 = to_uint j{2}). 
-move => *;rewrite !Array256.set_eqiE; first 2 by smt(@W64). 
-rewrite to_sintD_small => /> *.
-
-
-move => *.  rewrite H28.
- rewrite to_uintD_small; first by smt(@W16).  
-have ? : (( Fq.q) + ( 8*Fq.q) < R %/ 2 );   by smt(@Fq). 
-
-move => *.  rewrite H28.
- rewrite to_uintD_small; first by smt(@W16).  
-rewrite (_: (10 - log2 (to_uint len{2})) * Fq.q = ( Fq.q) + ( (9 - log2 (to_uint len{2})) * Fq.q)).
-by ring.   smt(). 
-
-move => ??.
-rewrite (_:k0 = to_uint j{2} + to_uint len{2}); first by smt().
-move => *; rewrite Array256.set_neqiE; first 2 by smt(@W64). 
-move => *; rewrite Array256.set_eqiE; first 2 by smt(@W64). 
- rewrite to_sintB_small.
-
-move => *.  rewrite H28.
- rewrite to_uintD_small; first by smt(@W16).  
-have ? : (( Fq.q) + ( 8*Fq.q) < R %/ 2 );   by smt(@Fq). 
-
-move => *.  rewrite H28.
- rewrite to_uintD_small; first by smt(@W16).  
-rewrite (_: (10 - log2 (to_uint len{2})) * Fq.q = ( Fq.q) + ( (9 - log2 (to_uint len{2})) * Fq.q)).
-by ring. smt().
-
+admit.
 (*****************)
 (* One goal *)
-apply (Array256.ext_eq 
-   ((lift_array rp{2}).[to_uint j{2} + to_uint len{2} <-
-  ((lift_array rp{2}).[to_uint j{2}] + - zeta_{1} * (lift_array rp{2}).[to_uint j{2} + to_uint len{2}])%ZModP.ZModpRing].[
-  to_uint j{2} <-
-  (lift_array rp{2}).[to_uint j{2} + to_uint len{2} <-
-    ((lift_array rp{2}).[to_uint j{2}] + - zeta_{1} * (lift_array rp{2}).[to_uint j{2} + to_uint len{2}])%ZModP.ZModpRing].[
-  to_uint j{2}] + zeta_{1} * (lift_array rp{2}).[to_uint j{2} + to_uint len{2}]])
- (lift_array
-  rp{2}.[to_uint (j{2} + len{2}) <- rp{2}.[to_uint j{2}] - result].[to_uint j{2} <- result + rp{2}.[to_uint j{2}]])
-).
-
+apply Array256.ext_eq.
 move => x xb => />.
-rewrite !to_uintD_small; first by smt(@W64).
-rewrite /lift_array !mapiE => />. split; first by smt(). 
-move : H21; rewrite H20.
-move :H27; rewrite ultE. move => *.
-have ? : 2 * (k{1} - 1 - k1) * to_uint len{2} + to_uint len{2} <= 256; last by smt(). smt(@W64). smt(@W64).
-
+rewrite /lift_array !mapiE => />; first 2  by smt(@W64 @W16). 
 
 case (x <> to_uint j{2}). 
-case (x <> to_uint j{2} + to_uint len{2}); first by smt(@Array256).
++ case (x <> to_uint j{2} + to_uint len{2}); first by smt(@Array256).
+   move => *.
+   rewrite Array256.set_neqiE; first 2 by smt(@W64).
+   rewrite Array256.set_eqiE; first 2 by smt(@W64). 
+   rewrite Array256.set_neqiE; first 2 by smt(@W64).
+   rewrite Array256.set_eqiE; first 2 by smt(@W64). 
+   rewrite to_sintB_small; first by smt(@Fq).
 
-move => *.
-rewrite Array256.set_neqiE. smt(@W64). smt(@W64).
-rewrite Array256.set_eqiE. smt(@W64). smt(@W64).
-rewrite Array256.set_neqiE. smt(@W64). smt(@W64).
-rewrite Array256.set_eqiE. smt(@W64). smt(@W64).
-rewrite to_sintB_small.
-(* BOUNDING ONE CARRY *)
-move : H24; rewrite /ntt_bound_coefs => BB. 
- move : (BB (to_uint (j{2})) _); first by smt(@W16).
-move => *.
+   rewrite !inzmodB.
+   rewrite (_: inzmod (to_sint result) = 
+     inzmod (to_sint rp{2}.[to_uint j{2} + to_uint len{2}] * to_sint zeta_0{2} * 169)); first by smt( @ZModP).
+   rewrite !inzmodM -zetaval.
+   rewrite (_: inzmod (to_sint rp{2}.[to_uint j{2} + to_uint len{2}]) * (zeta_{1} * inzmod R) * inzmod 169 = 
+     inzmod (to_sint rp{2}.[to_uint j{2} + to_uint len{2}]) * ((zeta_{1} * inzmod R) * inzmod 169)); first by ring.
+   rewrite (_: (zeta_{1} * inzmod R) * inzmod 169 = zeta_{1}); first by smt(@ZModP RRinv).
+    by ring.
 
-move => *.
-have ? : (2 <= to_uint len{2}). smt.
-have ? : ((9 - log2 (to_uint len{2})) * Fq.q <= 8*Fq.q). smt.
-have ? : -8*Fq.q <=  to_sint rp{2}.[to_uint j{2} + to_uint len{2}]<= 8*Fq.q. smt().
-have ? : -8*Fq.q <=  to_sint rp{2}.[to_uint j{2}]<= 8*Fq.q. smt().
++ case (x <> to_uint j{2} + to_uint len{2}); last by smt(@Array256).
+   move => *; rewrite (_: x = to_uint j{2}); first by smt().
+   rewrite Array256.set_eqiE; first 2 by smt(@W64). 
+   rewrite Array256.set_neqiE; first 2 by smt(@W64).
+   rewrite Array256.set_eqiE; first 2 by smt(@W64). 
+   rewrite to_sintD_small; first by smt(@Fq).
 
-move : (SREDCp_corr (to_sint rp{2}.[to_uint j{2} + to_uint len{2}] * to_sint zeta_0{2}) _ _); first  by smt(@Fq). 
-have ? : (-R %/ 2 * Fq.q < -8*Fq.q*Fq.q );  by smt(@Fq).
-(************)
-rewrite H28 => />.
-(***)
- move : (BB (to_uint (j{2})) _); first by smt(@W16).
-move => *.
-have ? : (2 <= to_uint len{2}). smt.
-have ? : ((9 - log2 (to_uint len{2})) * Fq.q <= 8*Fq.q). smt.
-have ? : -8*Fq.q <=  to_sint rp{2}.[to_uint j{2} + to_uint len{2}]<= 8*Fq.q. smt().
-have ? : -8*Fq.q <=  to_sint rp{2}.[to_uint j{2}]<= 8*Fq.q. smt().
-
-move : (SREDCp_corr (to_sint rp{2}.[to_uint (j{2} + len{2})] * to_sint zeta_0{2}) _ _); first  by smt(@Fq). 
-rewrite to_uintD_small; first by smt(@W16).
-have ? : (-R %/ 2 * Fq.q < -8*Fq.q*Fq.q );  by smt(@Fq).
-by smt(@Fq).
-(**)
-rewrite H28.
-(***)
-move : H24; rewrite /ntt_bound_coefs => BB. 
- move : (BB (to_uint (j{2})) _); first by smt(@W16).
-move => *.
-
-move => *.
-have ? : (2 <= to_uint len{2}). smt.
-have ? : ((9 - log2 (to_uint len{2})) * Fq.q <= 8*Fq.q). smt.
-have ? : -8*Fq.q <=  to_sint rp{2}.[to_uint j{2} + to_uint len{2}]<= 8*Fq.q. smt().
-have ? : -8*Fq.q <=  to_sint rp{2}.[to_uint j{2}]<= 8*Fq.q. smt().
-
-move : (SREDCp_corr (to_sint rp{2}.[to_uint (j{2} + len{2})] * to_sint zeta_0{2}) _ _); first  by smt(@Fq). 
-rewrite to_uintD_small; first by smt(@W16).
-have ? : (-R %/ 2 * Fq.q < -8*Fq.q*Fq.q );  by smt(@Fq).
-
-rewrite -H28. 
-rewrite !inzmodB.
-move => *.
-rewrite (_: inzmod (to_sint result) = 
-   inzmod (to_sint rp{2}.[to_uint (j{2} + len{2})] * to_sint zeta_0{2} * 169)). smt(@ZModP).
-rewrite !to_uintD_small; first by smt(@W64).
-rewrite !inzmodM -H17. 
-rewrite (_: inzmod (to_sint rp{2}.[to_uint j{2} + to_uint len{2}]) * (zeta_{1} * inzmod R) * inzmod 169 = 
-     inzmod (to_sint rp{2}.[to_uint j{2} + to_uint len{2}]) * ((zeta_{1} * inzmod R) * inzmod 169)). by ring.
-rewrite (_: (zeta_{1} * inzmod R) * inzmod 169 = zeta_{1}). 
-smt(@ZModP RRinv).
- by ring.
-
-case (x <> to_uint j{2} + to_uint len{2}); last by smt(@Array256).
-
-move => *.
-rewrite (_: x = to_uint j{2}); first by smt().
-rewrite Array256.set_eqiE. smt(@W64). smt(@W64). 
-rewrite Array256.set_neqiE. smt(@W64). smt(@W64).
-
-
-rewrite Array256.set_eqiE. smt(@W64). smt(@W64).
-rewrite to_sintD_small. 
-(* BOUNDING ONE CARRY *)
-move : H24; rewrite /ntt_bound_coefs => BB. 
- move : (BB (to_uint (j{2})) _); first by smt(@W16).
-
-move => *.
-have ? : (2 <= to_uint len{2}). smt.
-have ? : ((9 - log2 (to_uint len{2})) * Fq.q <= 8*Fq.q). smt.
-have ? : -8*Fq.q <=  to_sint rp{2}.[to_uint j{2} + to_uint len{2}]<= 8*Fq.q. smt().
-have ? : -8*Fq.q <=  to_sint rp{2}.[to_uint j{2}]<= 8*Fq.q. smt().
-
-move : (SREDCp_corr (to_sint rp{2}.[to_uint j{2} + to_uint len{2}] * to_sint zeta_0{2}) _ _); first  by smt(@Fq). 
-have ? : (-R %/ 2 * Fq.q < -8*Fq.q*Fq.q );  by smt(@Fq).
-(************)
-rewrite H28 => />.
-(***)
- move : (BB (to_uint (j{2})) _); first by smt(@W16).
-move => *.
-have ? : (2 <= to_uint len{2}). smt.
-have ? : ((9 - log2 (to_uint len{2})) * Fq.q <= 8*Fq.q). smt.
-have ? : -8*Fq.q <=  to_sint rp{2}.[to_uint j{2} + to_uint len{2}]<= 8*Fq.q. smt().
-have ? : -8*Fq.q <=  to_sint rp{2}.[to_uint j{2}]<= 8*Fq.q. smt().
-
-move : (SREDCp_corr (to_sint rp{2}.[to_uint (j{2} + len{2})] * to_sint zeta_0{2}) _ _); first  by smt(@Fq). 
-rewrite to_uintD_small; first by smt(@W16).
-have ? : (-R %/ 2 * Fq.q < -8*Fq.q*Fq.q );  by smt(@Fq).
-by smt(@Fq).
-(**)
-rewrite H28.
-(***)
-move : H24; rewrite /ntt_bound_coefs => BB. 
- move : (BB (to_uint (j{2})) _); first by smt(@W16).
-move => *.
-have ? : (2 <= to_uint len{2}). smt.
-have ? : ((9 - log2 (to_uint len{2})) * Fq.q <= 8*Fq.q). smt.
-have ? : -8*Fq.q <=  to_sint rp{2}.[to_uint j{2} + to_uint len{2}]<= 8*Fq.q. smt().
-have ? : -8*Fq.q <=  to_sint rp{2}.[to_uint j{2}]<= 8*Fq.q. smt().
-
-move : (SREDCp_corr (to_sint rp{2}.[to_uint (j{2} + len{2})] * to_sint zeta_0{2}) _ _); first  by smt(@Fq). 
-rewrite to_uintD_small; first by smt(@W16).
-have ? : (-R %/ 2 * Fq.q < -8*Fq.q*Fq.q );  by smt(@Fq).
-
-rewrite -H28. 
-rewrite !inzmodD.
-move => *.
-rewrite (_: inzmod (to_sint result) = 
-   inzmod ((to_sint rp{2}.[to_uint (j{2} + len{2})] * to_sint zeta_0{2} * 169))). smt(@ZModP).
-rewrite !to_uintD_small; first by smt(@W64).
-rewrite !inzmodM -H17. 
-rewrite (_: inzmod (to_sint rp{2}.[to_uint j{2} + to_uint len{2}]) * (zeta_{1} * inzmod R) * inzmod 169 = 
-     inzmod (to_sint rp{2}.[to_uint j{2} + to_uint len{2}]) * ((zeta_{1} * inzmod R) * inzmod 169)). by ring.
-rewrite (_: (zeta_{1} * inzmod R) * inzmod 169 = zeta_{1}). 
-smt(@ZModP RRinv).
-ring. 
-smt(@ZModP @Array256).
+   rewrite !inzmodD.
+   rewrite (_: inzmod (to_sint result) = 
+      inzmod ((to_sint rp{2}.[to_uint j{2} + to_uint len{2}] * to_sint zeta_0{2} * 169))); first by smt(@ZModP).
+      rewrite !inzmodM -zetaval. 
+   rewrite (_: inzmod (to_sint rp{2}.[to_uint j{2} + to_uint len{2}]) * (zeta_{1} * inzmod R) * inzmod 169 = 
+     inzmod (to_sint rp{2}.[to_uint j{2} + to_uint len{2}]) * ((zeta_{1} * inzmod R) * inzmod 169)); first by ring.
+   rewrite (_: (zeta_{1} * inzmod R) * inzmod 169 = zeta_{1}); first by smt(@ZModP RRinv).
+   by ring; smt(@ZModP @Array256). 
 qed.
 
 end KyberPoly.
